\pdfminorversion=4
\documentclass[]{article}

%%%%%%%%%%%%%%%%%%%
% Packages/Macros %
%%%%%%%%%%%%%%%%%%%
\usepackage{amssymb,latexsym,geometry,xcolor,framed,url,xr}     % Standard packages
\usepackage{amsmath}
\usepackage{colors}
%%%%%%%%%%%%
% Document %
%%%%%%%%%%%%
\newgeometry{left=1cm,top=1cm,right=1cm,bottom=2cm}
\begin{document}
\allowdisplaybreaks
\raggedbottom
\section*{Euler Project - Problem 6 - Appendix A}
\subsection*{Corollaries \& Identities}
\subsubsection*{Lemma 1}
Let $j$ be any natural number between $1$ and $N$. Then,
\[\sum_{i=1}^{N}=\sum_{i=1}^{j}i + \sum_{i=j+1}^{N}i\]\\
\textit{Proof:}\
The sum on the left may be written as:
\[1 + 2 + 3 + ... + N\]
Since $j$ is a natural number between $1$ and $N$, this is equivalent to: 
\[1 + 2 + ... + j + ... + N\]
As well as:
\[1 + 2 + ... + j + (j+1) + ... + N\]
Then, by associativity of addition in $\mathbb{R}$ (and consequently $\mathbb{N}$):
\[1 + 2 + ... + j + (j+1) + ... + N = (1 + 2 + ... + j) + ((j+1) + ... + N)\]
Which, writing the sequences as sums again, gives:
\[\sum_{i=1}^{N}=\sum_{i=1}^{j}i + \sum_{i=j+1}^{N}i\]

\subsubsection*{Corollary 1}
Rewriting the equation to express the third sum from the left gives:
\[\sum_{i=j+1}^{N}=\sum_{i=1}^{N}i-\sum_{i=1}^{j}i\]

\subsubsection*{Lemma 2.1}
Let $S$ be the sum of an arithmetic series of natural numbers from $1$ to $N$, where $N \in \mathbb{N}$. Then,
\[S=\sum_{i=1}^{N}=\frac{N(N+1)}{2}\]
\textit{Proof:} Recall the formula for the sum of an arithmetic series of the form:
\[\frac{n}{2}(a_1 + a_n)\]
where $n$ is the number of terms, $a_1$ is the first term, and $a_n$ is the last term.\\
Since the number of terms is $N$, which is also the last term, since the first term is $1$, then:
\[\frac{n}{2}(a_1 + a_n) = \frac{N}{2}(1 + N) = \frac{N(N+1)}{2}\]

\subsubsection*{Lemma 2.2}
Let $S$ be the sum of an arithmetic series of squared natural numbers from $1$ to $N$, where $N \in \mathbb{N}$. Then,
\[S=\sum_{i=1}^{N}i^2=\frac{N(N+1)(2N+1)}{6}\]
\textit{Proof:} A sample proof using mathematical induction may be found at: \url{https://www.youtube.com/watch?v=JiBd5yyYfUE}
\textit{Alternate proof:} An intuitive visual proof using 3D cubes may be seen at: \url{https://www.youtube.com/watch?v=aXbT37IlyZQ}
\subsubsection*{Lemma 2.3}
Let $S$ be the sum of an arithmetic series of cubed natural numbers from $1$ to $N$, where $N \in \mathbb{N}$. Then,
\[S=\sum_{i=1}^{N}i^3=\left(\sum_{i=1}^{N}i\right)^2=\left(\frac{N(N+1)}{2}\right)^2=\frac{N^2(N+1)^2}{4}\]
\textit{Proof:} A sample proof using mathematical induction may be found at: \url{https://www.youtube.com/watch?v=w362XRZy5as}
\textit{Alternate proof:} An intuitive visual proof once again using 3D cubes may be seen at: \url{https://www.youtube.com/watch?v=w362XRZy5as}
\end{document}
